value refactoring

deps/poulet4/lib/P4cub/Semantics/Dynamic/BigStep/Value/Auxilary.v
@@ -1,43 +1,73 @@
 Require Import Coq.NArith.BinNat
         Poulet4.P4cub.Semantics.Dynamic.BigStep.Value.Syntax
         Coq.PArith.BinPos Coq.ZArith.BinInt
-        Poulet4.P4cub.Syntax.CubNotations.
-Import Val ValueNotations AllCubNotations.
+        Poulet4.P4cub.Syntax.CubNotations
+        Poulet4.P4cub.Semantics.Static.Util
+        Poulet4.P4cub.Semantics.Static.IndPrincip
+        Poulet4.Utils.ForallMap
+        Poulet4.P4cub.Semantics.Dynamic.BigStep.Value.IndPrincip
+        (*Poulet4.P4cub.Syntax.IndPrincip*).
+Import Val ValueNotations ExprNotations ParserNotations.
+
+(* TODO: Also in [P4light/Semantics/Typing/Utility.v]
+   Should be moved to somewhere in [Utils]. *)
+Ltac some_inv :=
+  match goal with
+  | H: Some _ = Some _ |- _ => inv H
+  end.
+
+Ltac match_some_inv :=
+  match goal with
+  | H: match ?trm with Some _ => _ | None => _ end = Some _
+    |- _ => destruct trm as [? |] eqn:? ; cbn in *;
+          try discriminate
+  end.
+
+Local Open Scope value_scope.
+Local Open Scope type_scope.
 
 (** Intial/Default value from a type. *)
-Fixpoint vdefault (τ : Expr.t) : option v :=
+Fixpoint v_of_t (τ : Expr.t) : option v :=
   match τ with
-  | {{ error }}      => Some ~{ ERROR None }~
-  | {{ Bool }}       => Some ~{ FALSE }~
-  | {{ bit<w> }}     => Some $ VBit w 0%Z
-  | {{ int<w> }}     => Some $ VInt w 0%Z
-  | {{ tuple ts }}
-    => vs <<| sequence $ List.map vdefault ts ;; VTuple vs
-  | {{ struct { ts } }}
-    => vs <<| sequence $ List.map (fun '(x,t) => v <<| vdefault t ;; (x, v)) ts ;;
-      ~{ STRUCT { vs } }~
-  | {{ hdr { ts } }}
-    => vs <<| sequence $ List.map (fun '(x,t) => v <<| vdefault t ;; (x, v)) ts ;;
-      ~{ HDR { vs } VALID:=false }~
-  | {{ stack ts[n] }}
-    => vs <<| sequence $ List.map (fun '(x,t) => v <<| vdefault t ;; (x, v)) ts ;;
-      VHeaderStack ts (repeat (false, vs) (Pos.to_nat n)) 0
+  | Expr.TError => Some $ Error None
+  | Expr.TBool  => Some $ Bool false
+  | Expr.TBit w => Some $ Bit w 0%Z
+  | Expr.TInt w => Some $ Int w 0%Z
+  | Expr.TStruct ts b
+    => let^ vs := sequence $ List.map v_of_t ts in
+      Struct vs (if b then Some false else None)
   | Expr.TVar _ => None
   end.
-(**[]*)
+
+Lemma v_of_t_ok : forall τ, t_ok 0 τ -> exists V, v_of_t τ = Some V.
+Proof.
+  intros t h; remember 0%nat as z eqn:eqz.
+  induction h using custom_t_ok_ind; subst; unravel; eauto; try lia.
+  rewrite Forall_forall in H0.
+  pose proof (fun t hin => H0 t hin eq_refl) as ih; clear H0.
+  rewrite <- Forall_forall in ih.
+  rewrite Forall_exists_factor in ih.
+  destruct ih as [vs ih].
+  rewrite Forall2_map_l with
+    (f:=v_of_t) (R:=fun ov V => ov = Some V),
+      Forall2_sequence_iff in ih.
+  rewrite ih; eauto.
+Qed.
+
+Local Open Scope pat_scope.
 
 Fixpoint match_pattern (p : Parser.pat) (V : v) : bool :=
   match p, V with
-  | [{ ?? }], _ => true
-  | [{ (w PW a) &&& (_ PW b) }], ~{ _ VW c }~
+  | Parser.Wild, _ => true
+  | Parser.Mask (w PW a) (_ PW b), _ VW c
     => (Z.land a b =? Z.land c b)%Z
-  | [{ (w PW a) .. (_ PW b) }], ~{ _ VW c }~
+  | Parser.Range (w PW a) (_ PW b), _ VW c
     => (a <=? c)%Z && (c <=? b)%Z
-  | [{ w1 PW n1 }], ~{ w2 VW n2 }~ =>
+  | w1 PW n1, w2 VW n2 =>
     (w1 =? w2)%N && (n1 =? n2)%Z
-  | [{ w1 PS n1 }], ~{ w2 VS n2 }~ =>
-    (w1 =? w2)%positive && (n1 =? n2)%Z
-  | [{ PTUP ps }], ~{ TUPLE vs }~ =>
+  | w1 PS n1, w2 VS n2 =>
+    (w1 =? w2)%N && (n1 =? n2)%Z
+  | Parser.Struct ps, Struct vs None =>
     (fix F ps vs :=
        match ps, vs with
        | [], [] => true
@@ -46,46 +76,69 @@ Fixpoint match_pattern (p : Parser.pat) (V : v) : bool :=
        end) ps vs
   | _,_ => false
   end.
-(**[]*)
 
-Fixpoint approx_type (V : v) : Expr.t :=
+Fixpoint t_of_v (V : v) : Expr.t :=
   match V with
-  | ~{ VBOOL _ }~ => {{ Bool }}
-  | ~{ w VW _ }~ => {{ bit<w> }}
-  | ~{ w VS _ }~ => {{ int<w> }}
-  | ~{ ERROR _ }~ => {{ error }}
-  | ~{ TUPLE vs }~ => Expr.TTuple $ List.map approx_type vs
-  | ~{ STRUCT { vs } }~
-    => Expr.TStruct $ F.map approx_type vs
-  | ~{ HDR { vs } VALID:=_ }~
-    => Expr.THeader $ F.map approx_type vs
-  | ~{ STACK hs:ts NEXT:=_ }~ => Expr.THeaderStack ts (Pos.of_nat (length hs))
+  | Bool _ => Expr.TBool
+  | w VW _ => Expr.TBit w
+  | w VS _ => Expr.TInt w
+  | Error _ => Expr.TError
+  | Struct vs ob
+    => Expr.TStruct (List.map t_of_v vs) (if ob then true else false)
   end.
-(**[]*)
-                      
-Section Util.
-  Context {tags_t : Type}.
 
-  Variable i : tags_t.
-  
-  Fixpoint expr_of_value (V : v) : Expr.e tags_t :=
-    match V with
-    | ~{ VBOOL b }~ => <{ BOOL b @ i }>
-    | ~{ w VW n }~ => <{ w W n @ i }>
-    | ~{ w VS z }~ => <{ w S z @ i }>
-    | ~{ ERROR err }~ => <{ Error err @ i }>
-    | ~{ TUPLE vs }~
-      => Expr.ETuple (List.map expr_of_value vs) i
-    | ~{ STRUCT { vs } }~
-      => Expr.EStruct (F.map expr_of_value vs) i
-    | ~{ HDR { vs } VALID:=b }~
-      => Expr.EHeader (F.map expr_of_value vs) <{ BOOL b @ i }> i
-    | ~{ STACK hs:ts NEXT:=ni }~
-      => Expr.EHeaderStack
-          ts
-          (List.map
-             (fun '(b,vs) =>
-                Expr.EHeader
-                  (F.map expr_of_value vs) <{ BOOL b @ i }> i) hs) ni i
-    end.
-End Util.
+Lemma t_of_v_of_t : forall V τ,
+    v_of_t τ = Some V -> t_of_v V = τ.
+Proof.
+  intro V; induction V using custom_v_ind;
+    intros [] h; unravel in *;
+    try match_some_inv; try some_inv;
+    try (discriminate || reflexivity).
+  f_equal.
+  - generalize dependent fields.
+    clear isheader.
+    induction H as [| V vs h ih];
+      intros [| t ts] hs; cbn in *;
+      try (discriminate || reflexivity);
+      unfold option_bind in hs;
+      repeat match_some_inv. some_inv.
+    f_equal; auto.
+  - destruct isheader; reflexivity.
+Qed.
+
+Lemma t_of_v_of_t_ok : forall τ,
+    t_ok 0 τ ->
+    option_map t_of_v (v_of_t τ) = Some τ.
+Proof.
+  intros t h.
+  destruct (v_of_t_ok _ h) as [v hv].
+  rewrite hv; cbn; f_equal.
+  auto using t_of_v_of_t.
+Qed.
+
+Local Open Scope expr_scope.
+
+Fixpoint e_of_v (V : v) : Expr.e :=
+  match V with
+  | Bool b => Expr.Bool b
+  | w VW n => w `W n
+  | w VS z => w `S z
+  | Error err => Expr.Error err
+  | Struct vs ob
+    => Expr.Struct (map e_of_v vs) (option_map Expr.Bool ob)
+  end.
+
+Lemma t_of_e_of_v : forall V,
+    t_of_e (e_of_v V) = t_of_v V.
+Proof.
+  intro V; induction V using custom_v_ind;
+    unravel; try reflexivity; f_equal.
+  - apply map_ext_Forall in H.
+    rewrite map_map; assumption.
+  - destruct ob; reflexivity.
+Qed.
+
+Local Close Scope value_scope.
+Local Close Scope type_scope.
+Local Close Scope pat_scope.
+Local Close Scope expr_scope.
